EffectSSA/ProofSketch/Effect.lean
@@ -15,22 +15,24 @@ open ITree
 open Effect (trigger)
 open MonadIter (iter)
 
+variable {ε : Type} {κε : ε → Type} [Effect ε κε]
+         {δ : Type} {κδ : δ → Type} [Effect δ κδ]
+         {α : Type}
+
 /-!
 ## Errors / UB
 --------------------------------------------------------------------------------
 -/
 
-inductive ErrUBKind
-  | ub (reason : String)
-  | error (reason : String)
-
 /--
 `ErrUB` allows raising errors (which indicate a malformed program)
 as well as Undefined Behaviour.
 -/
-def ErrUB : ITree.Effect where
-  I := ErrUBKind
-  O _ := Empty
+inductive ErrUB
+  | ub (reason : String)
+  | error (reason : String)
+
+instance : Effect ErrUB (fun _ => Empty) := ⟨⟩
 
 /-! ### Helpers -/
 
@@ -49,7 +51,9 @@ def raiseError [ErrUB -< ε] (reason := "") : ITree ε α :=
 Let `SideEff` be some arbitrary set of language-specific side-effects.
 This could, e.g, model memory operations.
 -/
-axiom SideEff : ITree.Effect
+axiom SideEff : Type
+axiom SideEff.κ : SideEff → Type
+instance : Effect SideEff SideEff.κ := ⟨⟩
 
 /-!
 ## Hole Execution
@@ -69,9 +73,9 @@ Note that although holes in the AST have an intrinsically typed upper bound,
 `HoleEff` carries only the raw `Nat`-typed id of the hole, to prevent too many
 dependent types showing up in the semantics.
 -/
-def HoleEff : ITree.Effect where
-  I := HoleId
-  O _ := Unit
+abbrev HoleEff := HoleId
+
+instance : Effect HoleEff (fun _ => Unit) := ⟨⟩
 
 /-! ### Helper -/
 
@@ -83,7 +87,7 @@ def jumpToHole (h : HoleId) : ITree HoleEff Unit :=
 
 /-- Interpret hole effects by delegating each hole id to `f`. -/
 def interpHoles [ε -< δ] (f : HoleId → ITree ε Unit) :
-    (x : ITree (HoleEff ⊕ₑ δ) α) → ITree δ α :=
+    (x : ITree (HoleEff ⊕ δ) α) → ITree δ α :=
   ITree.interpLeft (f · |>.lift)
 
 /--
@@ -93,7 +97,7 @@ It can be used to avoid having to specify `ε` when Lean fails to infer it.
 -/
 @[simp, grind]
 abbrev interpHoles'  : (f : HoleId → ITree δ Unit) →
-    (x : ITree (HoleEff ⊕ₑ δ) α) → ITree δ α :=
+    (x : ITree (HoleEff ⊕ δ) α) → ITree δ α :=
   interpHoles
 
 /-!
@@ -109,23 +113,21 @@ instance : ToString VarId where toString := VarId.raw
 /-- `Val` is the type of runtime values -/
 axiom Val : Type
 
-inductive LocalEffKind
+inductive LocalEff
   | read (var : VarId)
   | push (var : VarId) (value : Val)
 
-def LocalEff : ITree.Effect where
-  I := LocalEffKind
-  O := fun
+instance : Effect LocalEff (fun
     | .read _ => Val
-    | .push _ _ => Unit
+    | .push _ _ => Unit) := ⟨⟩
 
 /-! ### Helpers -/
 
 def readVar [LocalEff -< ε] (var : VarId) : ITree ε Val :=
-  trigger (E₁ := LocalEff) <| .read var
+  trigger LocalEff <| .read var
 
 def pushVar [LocalEff -< ε] (var : VarId) (value : Val) : ITree ε Unit :=
-  trigger (E₁ := LocalEff) <| .push var value
+  trigger LocalEff <| .push var value
 
 /-! ### Interpretation -/
 
@@ -133,7 +135,7 @@ structure LocalStack where
   raw : Std.HashMap VarId Val := { }
 
 def interpLocalStackM [ErrUB -< ε] :
-    (x : ITree (LocalEff ⊕ₑ ε) α) → StateT LocalStack (ITree ε) α :=
+    (x : ITree (LocalEff ⊕ ε) α) → StateT LocalStack (ITree ε) α :=
   ITree.interpM fun
     | .inr e => liftM <| ITree.vis e .ret
     | .inl (.read x) => do
@@ -150,7 +152,7 @@ def interpLocalStackM [ErrUB -< ε] :
         -- a previous iteration of a loop.
 
 /-- Interpret local stack effects starting from an empty initial stack. -/
-def interpLocalStack [ErrUB -< ε] (x : ITree (LocalEff ⊕ₑ ε) α) : ITree ε α :=
+def interpLocalStack [ErrUB -< ε] (x : ITree (LocalEff ⊕ ε) α) : ITree ε α :=
   (interpLocalStackM x).run' { }
 
 /-!
@@ -168,9 +170,9 @@ structure right away.
 -/
 
 /-- In `InstEff`, each instruction is a unique effect. -/
-def InstEff : ITree.Effect where
-  I := Inst
-  O _ := Unit
+abbrev InstEff := Inst
+
+instance : Effect InstEff (fun _ => Unit) := ⟨⟩
 
 /-! ### Handler -/
 
@@ -178,5 +180,5 @@ axiom handleInst [ErrUB -< ε] [SideEff -< ε] [LocalEff -< ε] : (i : Inst) →
 
 noncomputable
 def interpInst [ErrUB -< ε] [SideEff -< ε] [LocalEff -< ε] :
-    ITree (InstEff ⊕ₑ ε) α → ITree ε α :=
+    ITree (InstEff ⊕ ε) α → ITree ε α :=
   ITree.interpLeft handleInst
